compiler/core/Driver/CompDriver.v
@@ -66,8 +66,8 @@ Require Import NRAtocNRAEnv.
 Require Import NNRCtocNNRC.
 Require Import NNRCtoNNRS.
 Require Import NNRStoNNRSimp.
-Require Import NNRSimptoImpQcert.
-Require Import ImpQcerttoImpEJson.
+Require Import NNRSimptoImpData.
+Require Import ImpDatatoImpEJson.
 Require Import ImpEJsontoJavaScriptAst.
 Require Import JavaScriptAsttoJavaScript.
 Require Import NNRCtoDNNRC.
@@ -205,12 +205,12 @@ Section CompDriver.
     Definition nnrs_to_nnrs_imp (q: nnrs) : nnrs_imp :=
       nnrs_to_nnrs_imp_top "$"%string q.
 
-    Definition nnrs_imp_to_imp_qcert (qname: string) (q: nnrs_imp) : imp_qcert :=
-      nnrs_imp_to_imp_qcert_top qname q.
+    Definition nnrs_imp_to_imp_data (qname: string) (q: nnrs_imp) : imp_data :=
+      nnrs_imp_to_imp_data_top qname q.
 
-    Definition imp_qcert_to_imp_ejson (q: imp_qcert) : imp_ejson :=
+    Definition imp_data_to_imp_ejson (q: imp_data) : imp_ejson :=
       (* Note: Obtain brand relation from brand model, baked in imp_ejson compilation *)
-      imp_qcert_to_imp_ejson brand_relation_brands q.
+      imp_data_to_imp_ejson brand_relation_brands q.
 
     Definition imp_ejson_to_js_ast (cname:option string) (q: imp_ejson) : js_ast :=
       imp_ejson_to_js_ast cname q.
@@ -302,15 +302,15 @@ Section CompDriver.
     | Dv_imp_ejson_to_js_ast : option string -> js_ast_driver -> imp_ejson_driver
   .
 
-  Inductive imp_qcert_driver : Set :=
-    | Dv_imp_qcert_stop : imp_qcert_driver
-    | Dv_imp_qcert_to_imp_ejson : imp_ejson_driver -> imp_qcert_driver
+  Inductive imp_data_driver : Set :=
+    | Dv_imp_data_stop : imp_data_driver
+    | Dv_imp_data_to_imp_ejson : imp_ejson_driver -> imp_data_driver
   .
 
   Inductive nnrs_imp_driver : Set :=
     | Dv_nnrs_imp_stop : nnrs_imp_driver
     | Dv_nnrs_imp_optim : optim_phases3_config -> nnrs_imp_driver -> nnrs_imp_driver
-    | Dv_nnrs_imp_to_imp_qcert : (* query name*) string -> imp_qcert_driver -> nnrs_imp_driver
+    | Dv_nnrs_imp_to_imp_data : (* query name*) string -> imp_data_driver -> nnrs_imp_driver
   .
 
   Inductive nnrs_driver : Set :=
@@ -438,7 +438,7 @@ Section CompDriver.
   | Dv_nnrs_core : nnrs_core_driver -> driver
   | Dv_nnrs : nnrs_driver -> driver
   | Dv_nnrs_imp : nnrs_imp_driver -> driver
-  | Dv_imp_qcert : imp_qcert_driver -> driver
+  | Dv_imp_data : imp_data_driver -> driver
   | Dv_imp_ejson : imp_ejson_driver -> driver
   | Dv_nnrcmr : nnrcmr_driver -> driver
   | Dv_dnnrc : dnnrc_driver -> driver
@@ -467,7 +467,7 @@ Section CompDriver.
     | Case_aux c "Dv_nnrs_core"%string
     | Case_aux c "Dv_nnrs"%string
     | Case_aux c "Dv_nnrs_imp"%string
-    | Case_aux c "Dv_imp_qcert"%string
+    | Case_aux c "Dv_imp_data"%string
     | Case_aux c "Dv_imp_ejson"%string
     | Case_aux c "Dv_nnrcmr"%string
     | Case_aux c "Dv_dnnrc"%string
@@ -492,7 +492,7 @@ Section CompDriver.
     | Dv_nnrs_core _ => L_nnrs_core
     | Dv_nnrs _ => L_nnrs
     | Dv_nnrs_imp _ => L_nnrs_imp
-    | Dv_imp_qcert _ => L_imp_qcert
+    | Dv_imp_data _ => L_imp_data
     | Dv_imp_ejson _ => L_imp_ejson
     | Dv_nnrcmr _ => L_nnrcmr
     | Dv_camp_rule _ => L_camp_rule
@@ -542,17 +542,17 @@ Section CompDriver.
     | Dv_imp_ejson_to_js_ast _ dv => 1 + driver_length_js_ast dv
     end.
 
-  Fixpoint driver_length_imp_qcert (dv: imp_qcert_driver) :=
+  Fixpoint driver_length_imp_data (dv: imp_data_driver) :=
     match dv with
-    | Dv_imp_qcert_stop => 1
-    | Dv_imp_qcert_to_imp_ejson dv => 1 + driver_length_imp_ejson dv
+    | Dv_imp_data_stop => 1
+    | Dv_imp_data_to_imp_ejson dv => 1 + driver_length_imp_ejson dv
     end.
 
   Fixpoint driver_length_nnrs_imp (dv: nnrs_imp_driver) :=
     match dv with
     | Dv_nnrs_imp_stop => 1
     | Dv_nnrs_imp_optim _ dv => 1 + driver_length_nnrs_imp dv
-    | Dv_nnrs_imp_to_imp_qcert _ dv => 1 + driver_length_imp_qcert dv
+    | Dv_nnrs_imp_to_imp_data _ dv => 1 + driver_length_imp_data dv
     end.
 
   Definition driver_length_nnrs (dv: nnrs_driver) :=
@@ -698,7 +698,7 @@ Section CompDriver.
     | Dv_nnrs_core dv => driver_length_nnrs_core dv
     | Dv_nnrs dv => driver_length_nnrs dv
     | Dv_nnrs_imp dv => driver_length_nnrs_imp dv
-    | Dv_imp_qcert dv => driver_length_imp_qcert dv
+    | Dv_imp_data dv => driver_length_imp_data dv
     | Dv_imp_ejson dv => driver_length_imp_ejson dv
     | Dv_nnrcmr dv => driver_length_nnrcmr dv
     | Dv_dnnrc dv => driver_length_dnnrc dv
@@ -760,16 +760,16 @@ Section CompDriver.
       in
       (Q_imp_ejson q) :: queries.
 
-    Definition compile_imp_qcert (dv: imp_qcert_driver) (q: imp_qcert) : list query :=
+    Definition compile_imp_data (dv: imp_data_driver) (q: imp_data) : list query :=
       let queries :=
           match dv with
-          | Dv_imp_qcert_stop => nil
-          | Dv_imp_qcert_to_imp_ejson dv =>
-            let q := imp_qcert_to_imp_ejson q in
+          | Dv_imp_data_stop => nil
+          | Dv_imp_data_to_imp_ejson dv =>
+            let q := imp_data_to_imp_ejson q in
             compile_imp_ejson dv q
           end
       in
-      (Q_imp_qcert q) :: queries.
+      (Q_imp_data q) :: queries.
 
     Fixpoint compile_nnrs_imp (dv: nnrs_imp_driver) (q: nnrs_imp) : list query :=
       let queries :=
@@ -778,9 +778,9 @@ Section CompDriver.
           | Dv_nnrs_imp_optim oc dv =>
             let q := nnrs_imp_optim oc q in
             compile_nnrs_imp dv q
-          | Dv_nnrs_imp_to_imp_qcert qname dv =>
-            let q := nnrs_imp_to_imp_qcert qname q in
-            compile_imp_qcert dv q
+          | Dv_nnrs_imp_to_imp_data qname dv =>
+            let q := nnrs_imp_to_imp_data qname q in
+            compile_imp_data dv q
           end
       in
       (Q_nnrs_imp q) :: queries.
@@ -1061,7 +1061,7 @@ Section CompDriver.
       | (Dv_nnrs_core dv, Q_nnrs_core q) => compile_nnrs_core dv q
       | (Dv_nnrs dv, Q_nnrs q) => compile_nnrs dv q
       | (Dv_nnrs_imp dv, Q_nnrs_imp q) => compile_nnrs_imp dv q
-      | (Dv_imp_qcert dv, Q_imp_qcert q) => compile_imp_qcert dv q
+      | (Dv_imp_data dv, Q_imp_data q) => compile_imp_data dv q
       | (Dv_imp_ejson dv, Q_imp_ejson q) => compile_imp_ejson dv q
       | (Dv_nnrcmr dv, Q_nnrcmr q) => compile_nnrcmr dv q
       | (Dv_dnnrc dv, Q_dnnrc q) => compile_dnnrc dv q
@@ -1098,7 +1098,7 @@ Section CompDriver.
       | Dv_nnrs_core _
       | Dv_nnrs _
       | Dv_nnrs_imp _
-      | Dv_imp_qcert _
+      | Dv_imp_data _
       | Dv_imp_ejson _
       | Dv_nnrcmr _
       | Dv_dnnrc _
@@ -1129,7 +1129,7 @@ Section CompDriver.
       | Dv_nnrs_core _
       | Dv_nnrs _
       | Dv_nnrs_imp _
-      | Dv_imp_qcert _
+      | Dv_imp_data _
       | Dv_imp_ejson _
       | Dv_nnrcmr _
       | Dv_dnnrc _
@@ -1160,7 +1160,7 @@ Section CompDriver.
       | Dv_nnrs_core _
       | Dv_nnrs _
       | Dv_nnrs_imp _
-      | Dv_imp_qcert _
+      | Dv_imp_data _
       | Dv_imp_ejson _
       | Dv_nnrcmr _
       | Dv_dnnrc _
@@ -1191,7 +1191,7 @@ Section CompDriver.
       | Dv_nnrs_core _
       | Dv_nnrs _
       | Dv_nnrs_imp _
-      | Dv_imp_qcert _
+      | Dv_imp_data _
       | Dv_imp_ejson _
       | Dv_nnrcmr _
       | Dv_dnnrc _
@@ -1222,7 +1222,7 @@ Section CompDriver.
       | Dv_nnrs_core _
       | Dv_nnrs _
       | Dv_nnrs_imp _
-      | Dv_imp_qcert _
+      | Dv_imp_data _
       | Dv_imp_ejson _
       | Dv_nnrcmr _
       | Dv_dnnrc _
@@ -1253,7 +1253,7 @@ Section CompDriver.
       | Dv_nnrs_core _
       | Dv_nnrs _
       | Dv_nnrs_imp _
-      | Dv_imp_qcert _
+      | Dv_imp_data _
       | Dv_imp_ejson _
       | Dv_nnrcmr _
       | Dv_dnnrc _
@@ -1284,7 +1284,7 @@ Section CompDriver.
       | Dv_nnrs_core _
       | Dv_nnrs _
       | Dv_nnrs_imp _
-      | Dv_imp_qcert _
+      | Dv_imp_data _
       | Dv_imp_ejson _
       | Dv_nnrcmr _
       | Dv_dnnrc _
@@ -1315,7 +1315,7 @@ Section CompDriver.
       | Dv_nnrs_core _
       | Dv_nnrs _
       | Dv_nnrs_imp _
-      | Dv_imp_qcert _
+      | Dv_imp_data _
       | Dv_imp_ejson _
       | Dv_nnrcmr _
       | Dv_dnnrc _
@@ -1346,7 +1346,7 @@ Section CompDriver.
       | Dv_nnrs_core _
       | Dv_nnrs _
       | Dv_nnrs_imp _
-      | Dv_imp_qcert _
+      | Dv_imp_data _
       | Dv_imp_ejson _
       | Dv_nnrcmr _
       | Dv_dnnrc _
@@ -1377,7 +1377,7 @@ Section CompDriver.
       | Dv_nnrs_core _
       | Dv_nnrs _
       | Dv_nnrs_imp _
-      | Dv_imp_qcert _
+      | Dv_imp_data _
       | Dv_imp_ejson _
       | Dv_nnrcmr _
       | Dv_dnnrc _
@@ -1408,7 +1408,7 @@ Section CompDriver.
       | Dv_nnrs_core _
       | Dv_nnrs _
       | Dv_nnrs_imp _
-      | Dv_imp_qcert _
+      | Dv_imp_data _
       | Dv_imp_ejson _
       | Dv_nnrcmr _
       | Dv_dnnrc _
@@ -1430,7 +1430,7 @@ Section CompDriver.
       | Dv_nraenv _
       | Dv_nnrs _
       | Dv_nnrs_imp _
-      | Dv_imp_qcert _
+      | Dv_imp_data _
       | Dv_imp_ejson _
       | Dv_nnrcmr _
       | Dv_dnnrc _
@@ -1472,7 +1472,7 @@ Section CompDriver.
       | Dv_lambda_nra _
       | Dv_nnrs_core _
       | Dv_nnrs_imp _
-      | Dv_imp_qcert _
+      | Dv_imp_data _
       | Dv_imp_ejson _
       | Dv_js_ast _
       | Dv_nra _
@@ -1501,7 +1501,7 @@ Section CompDriver.
       | Dv_nnrc _
       | Dv_nnrs_core _
       | Dv_nnrs_imp _
-      | Dv_imp_qcert _
+      | Dv_imp_data _
       | Dv_imp_ejson _
       | Dv_nnrcmr _
       | Dv_dnnrc _
@@ -1532,7 +1532,7 @@ Section CompDriver.
       | Dv_nnrc _
       | Dv_nnrs_core _
       | Dv_nnrs _
-      | Dv_imp_qcert _
+      | Dv_imp_data _
       | Dv_imp_ejson _
       | Dv_js_ast _
       | Dv_nnrcmr _
@@ -1547,7 +1547,7 @@ Section CompDriver.
       end
     | L_nnrs_imp =>
       match dv with
-      | Dv_imp_qcert dv => Dv_nnrs_imp (Dv_nnrs_imp_to_imp_qcert config.(comp_qname_lowercase) dv)
+      | Dv_imp_data dv => Dv_nnrs_imp (Dv_nnrs_imp_to_imp_data config.(comp_qname_lowercase) dv)
       | Dv_nnrs_imp dv => Dv_nnrs_imp (Dv_nnrs_imp_optim (get_optim_config L_nnrs_imp config.(comp_optim_config)) dv)
       | Dv_camp _
       | Dv_nraenv_core _
@@ -1576,12 +1576,12 @@ Section CompDriver.
       | Dv_error err =>
           Dv_error ("Cannot compile to error ("++err++")")
       end
-    | L_imp_qcert =>
+    | L_imp_data =>
       match dv with
-      | Dv_imp_qcert _ =>
-          Dv_error ("XXX TODO: imp_qcert optimizer XXX")
+      | Dv_imp_data _ =>
+          Dv_error ("XXX TODO: imp_data optimizer XXX")
       | Dv_imp_ejson dv =>
-        Dv_imp_qcert (Dv_imp_qcert_to_imp_ejson dv)
+        Dv_imp_data (Dv_imp_data_to_imp_ejson dv)
       | Dv_camp _
       | Dv_nraenv_core _
       | Dv_nraenv _
@@ -1612,7 +1612,7 @@ Section CompDriver.
     | L_imp_ejson =>
       match dv with
       | Dv_imp_ejson _ =>
-          Dv_error ("XXX TODO: imp_qcert optimizer XXX")
+          Dv_error ("XXX TODO: imp_data optimizer XXX")
       | Dv_js_ast dv =>
         Dv_imp_ejson (Dv_imp_ejson_to_js_ast config.(comp_class_name) dv)
       | Dv_camp _
@@ -1631,7 +1631,7 @@ Section CompDriver.
       | Dv_nnrs_core _
       | Dv_nnrs _
       | Dv_nnrs_imp _
-      | Dv_imp_qcert _
+      | Dv_imp_data _
       | Dv_nnrcmr _
       | Dv_dnnrc _
       | Dv_dnnrc_typed _
@@ -1652,7 +1652,7 @@ Section CompDriver.
       | Dv_nnrs_core _
       | Dv_nnrs _
       | Dv_nnrs_imp _
-      | Dv_imp_qcert _
+      | Dv_imp_data _
       | Dv_imp_ejson _
       | Dv_camp_rule _
       | Dv_tech_rule _
@@ -1694,7 +1694,7 @@ Section CompDriver.
       | Dv_nnrs_core _
       | Dv_nnrs _
       | Dv_nnrs_imp _
-      | Dv_imp_qcert _
+      | Dv_imp_data _
       | Dv_imp_ejson _
       | Dv_nnrcmr _
       | Dv_js_ast _
@@ -1727,7 +1727,7 @@ Section CompDriver.
       | Dv_nnrs_core _
       | Dv_nnrs _
       | Dv_nnrs_imp _
-      | Dv_imp_qcert _
+      | Dv_imp_data _
       | Dv_imp_ejson _
       | Dv_nnrcmr _
       | Dv_dnnrc _
@@ -1758,7 +1758,7 @@ Section CompDriver.
       | Dv_nnrs_core _
       | Dv_nnrs _
       | Dv_nnrs_imp _
-      | Dv_imp_qcert _
+      | Dv_imp_data _
       | Dv_imp_ejson _
       | Dv_nnrcmr _
       | Dv_dnnrc _
@@ -1796,7 +1796,7 @@ Section CompDriver.
     | L_nnrs_core => Dv_nnrs_core Dv_nnrs_core_stop
     | L_nnrs => Dv_nnrs Dv_nnrs_stop
     | L_nnrs_imp => Dv_nnrs_imp Dv_nnrs_imp_stop
-    | L_imp_qcert => Dv_imp_qcert Dv_imp_qcert_stop
+    | L_imp_data => Dv_imp_data Dv_imp_data_stop
     | L_imp_ejson => Dv_imp_ejson Dv_imp_ejson_stop
     | L_nnrcmr => Dv_nnrcmr Dv_nnrcmr_stop
     | L_dnnrc => Dv_dnnrc Dv_dnnrc_stop
@@ -1884,7 +1884,7 @@ Section CompDriver.
           True (* inputs = (vars_of_constants_config config.(comp_constants)) *)
         | Dv_nnrs_imp (Dv_nnrs_imp_optim opc _) =>
           opc = (get_optim_config L_nnrs_imp config.(comp_optim_config))
-        | Dv_nnrs_imp (Dv_nnrs_imp_to_imp_qcert qname _) =>
+        | Dv_nnrs_imp (Dv_nnrs_imp_to_imp_data qname _) =>
           qname = config.(comp_qname_lowercase)
         | Dv_dnnrc (Dv_dnnrc_to_dnnrc_typed tdbindings _) =>
           tdbindings = tdbindings_of_constants_config config.(comp_constants)
@@ -1957,9 +1957,9 @@ Section CompDriver.
     | Dv_nnrs (Dv_nnrs_to_nnrs_imp dv) => (L_nnrs, Some (Dv_nnrs_imp dv))
     | Dv_nnrs_imp (Dv_nnrs_imp_stop) => (L_nnrs_imp, None)
     | Dv_nnrs_imp (Dv_nnrs_imp_optim _ dv) => (L_nnrs_imp, Some (Dv_nnrs_imp dv))
-    | Dv_nnrs_imp (Dv_nnrs_imp_to_imp_qcert _ dv) => (L_nnrs_imp, Some (Dv_imp_qcert dv))
-    | Dv_imp_qcert (Dv_imp_qcert_stop) => (L_imp_qcert, None)
-    | Dv_imp_qcert (Dv_imp_qcert_to_imp_ejson dv) => (L_imp_qcert, Some (Dv_imp_ejson dv))
+    | Dv_nnrs_imp (Dv_nnrs_imp_to_imp_data _ dv) => (L_nnrs_imp, Some (Dv_imp_data dv))
+    | Dv_imp_data (Dv_imp_data_stop) => (L_imp_data, None)
+    | Dv_imp_data (Dv_imp_data_to_imp_ejson dv) => (L_imp_data, Some (Dv_imp_ejson dv))
     | Dv_imp_ejson (Dv_imp_ejson_stop) => (L_imp_ejson, None)
     | Dv_imp_ejson (Dv_imp_ejson_to_js_ast _ dv) => (L_imp_ejson, Some (Dv_js_ast dv))
     | Dv_nnrcmr (Dv_nnrcmr_stop) => (L_nnrcmr, None)
@@ -2101,8 +2101,8 @@ Section CompDriver.
       ; [eapply target_language_of_driver_is_postfix_js_ast | | ]; simpl; trivial.
   Qed.
 
-  Lemma target_language_of_driver_is_postfix_imp_qcert:
-    (forall dv, is_postfix_driver (driver_of_language (target_language_of_driver (Dv_imp_qcert dv))) (Dv_imp_qcert dv)).
+  Lemma target_language_of_driver_is_postfix_imp_data:
+    (forall dv, is_postfix_driver (driver_of_language (target_language_of_driver (Dv_imp_data dv))) (Dv_imp_data dv)).
   Proof.
     induction dv; simpl.
     - reflexivity.
@@ -2116,7 +2116,7 @@ Section CompDriver.
                  EmptyString
                  nil
                  EmptyString
-                 nil) (lang:=L_imp_qcert)
+                 nil) (lang:=L_imp_data)
       ; [eapply target_language_of_driver_is_postfix_imp_ejson | | ]; simpl; trivial.
   Qed.
 
@@ -2148,7 +2148,7 @@ Section CompDriver.
                  nil
                  EmptyString
                  nil) (lang:=L_nnrs_imp)
-      ; [eapply target_language_of_driver_is_postfix_imp_qcert | | ]; simpl; trivial.
+      ; [eapply target_language_of_driver_is_postfix_imp_data | | ]; simpl; trivial.
   Qed.
 
   Lemma target_language_of_driver_is_postfix_nnrs:
@@ -2507,7 +2507,7 @@ Section CompDriver.
          target_language_of_driver_is_postfix_nnrs_core
          target_language_of_driver_is_postfix_nnrs
          target_language_of_driver_is_postfix_nnrs_imp
-         target_language_of_driver_is_postfix_imp_qcert
+         target_language_of_driver_is_postfix_imp_data
          target_language_of_driver_is_postfix_imp_ejson
          target_language_of_driver_is_postfix_nnrcmr
          target_language_of_driver_is_postfix_camp_rule
@@ -2590,7 +2590,7 @@ Section CompDriver.
           rewrite H0; rewrite H3; reflexivity.
         * destruct (H_config (Dv_nnrs_imp (Dv_nnrs_imp_optim (get_optim_config L_nnrs_imp (comp_optim_config config0)) n)))
           ; try reflexivity.
-        * destruct (H_config (Dv_nnrs_imp (Dv_nnrs_imp_to_imp_qcert config0.(comp_qname_lowercase) i)));
+        * destruct (H_config (Dv_nnrs_imp (Dv_nnrs_imp_to_imp_data config0.(comp_qname_lowercase) i)));
             try reflexivity.
         * destruct (H_config (Dv_imp_ejson (Dv_imp_ejson_to_js_ast config0.(comp_class_name) j)));
             try reflexivity.
@@ -2683,7 +2683,7 @@ Section CompDriver.
           :: L_nnrs
           :: L_nnrs_imp
           :: L_nnrs_imp
-          :: L_imp_qcert
+          :: L_imp_data
           :: L_imp_ejson
           :: L_js_ast
           :: L_javascript
@@ -2727,7 +2727,7 @@ Section CompDriver.
           :: L_nnrs_imp
           :: L_nnrs_imp
           :: nil
-      | L_camp_rule, L_imp_qcert =>
+      | L_camp_rule, L_imp_data =>
         L_camp_rule
           :: L_camp
           :: L_nraenv
@@ -2737,7 +2737,7 @@ Section CompDriver.
           :: L_nnrs
           :: L_nnrs_imp
           :: L_nnrs_imp
-          :: L_imp_qcert
+          :: L_imp_data
           :: nil
       | L_camp_rule, L_imp_ejson =>
         L_camp_rule
@@ -2749,7 +2749,7 @@ Section CompDriver.
           :: L_nnrs
           :: L_nnrs_imp
           :: L_nnrs_imp
-          :: L_imp_qcert
+          :: L_imp_data
           :: L_imp_ejson
           :: nil
       | L_camp_rule, L_js_ast =>
@@ -2762,7 +2762,7 @@ Section CompDriver.
           :: L_nnrs
           :: L_nnrs_imp
           :: L_nnrs_imp
-          :: L_imp_qcert
+          :: L_imp_data
           :: L_imp_ejson
           :: L_js_ast
           :: nil
@@ -2870,7 +2870,7 @@ Section CompDriver.
           :: L_nnrs
           :: L_nnrs_imp
           :: L_nnrs_imp
-          :: L_imp_qcert
+          :: L_imp_data
           :: L_imp_ejson
           :: L_js_ast
           :: L_javascript
@@ -2918,7 +2918,7 @@ Section CompDriver.
           :: L_nnrs_imp
           :: L_nnrs_imp
           :: nil
-      | L_tech_rule, L_imp_qcert =>
+      | L_tech_rule, L_imp_data =>
         L_tech_rule
           :: L_camp_rule
           :: L_camp
@@ -2929,7 +2929,7 @@ Section CompDriver.
           :: L_nnrs
           :: L_nnrs_imp
           :: L_nnrs_imp
-          :: L_imp_qcert
+          :: L_imp_data
           :: nil
       | L_tech_rule, L_imp_ejson =>
         L_tech_rule
@@ -2942,7 +2942,7 @@ Section CompDriver.
           :: L_nnrs
           :: L_nnrs_imp
           :: L_nnrs_imp
-          :: L_imp_qcert
+          :: L_imp_data
           :: L_imp_ejson
           :: nil
       | L_tech_rule, L_js_ast =>
@@ -2956,7 +2956,7 @@ Section CompDriver.
           :: L_nnrs
           :: L_nnrs_imp
           :: L_nnrs_imp
-          :: L_imp_qcert
+          :: L_imp_data
           :: L_imp_ejson
           :: L_js_ast
           :: nil
@@ -3068,7 +3068,7 @@ Section CompDriver.
           :: L_nnrs
           :: L_nnrs_imp
           :: L_nnrs_imp
-          :: L_imp_qcert
+          :: L_imp_data
           :: L_imp_ejson
           :: L_js_ast
           :: L_javascript
@@ -3116,7 +3116,7 @@ Section CompDriver.
           :: L_nnrs_imp
           :: L_nnrs_imp
           :: nil
-      | L_designer_rule, L_imp_qcert =>
+      | L_designer_rule, L_imp_data =>
         L_designer_rule
           :: L_camp_rule
           :: L_camp
@@ -3127,7 +3127,7 @@ Section CompDriver.
           :: L_nnrs
           :: L_nnrs_imp
           :: L_nnrs_imp
-          :: L_imp_qcert
+          :: L_imp_data
           :: nil
       | L_designer_rule, L_imp_ejson =>
         L_designer_rule
@@ -3140,7 +3140,7 @@ Section CompDriver.
           :: L_nnrs
           :: L_nnrs_imp
           :: L_nnrs_imp
-          :: L_imp_qcert
+          :: L_imp_data
           :: L_imp_ejson
           :: nil
       | L_designer_rule, L_js_ast =>
@@ -3154,7 +3154,7 @@ Section CompDriver.
           :: L_nnrs
           :: L_nnrs_imp
           :: L_nnrs_imp
-          :: L_imp_qcert
+          :: L_imp_data
           :: L_imp_ejson
           :: L_js_ast
           :: nil
@@ -3245,7 +3245,7 @@ Section CompDriver.
           :: L_nnrs
           :: L_nnrs_imp
           :: L_nnrs_imp
-          :: L_imp_qcert
+          :: L_imp_data
           :: L_imp_ejson
           :: L_js_ast
           :: L_javascript
@@ -3285,7 +3285,7 @@ Section CompDriver.
           :: L_nnrs_imp
           :: L_nnrs_imp
           :: nil
-      | L_camp, L_imp_qcert =>
+      | L_camp, L_imp_data =>
         L_camp
           :: L_nraenv
           :: L_nraenv
@@ -3294,7 +3294,7 @@ Section CompDriver.
           :: L_nnrs
           :: L_nnrs_imp
           :: L_nnrs_imp
-          :: L_imp_qcert
+          :: L_imp_data
           :: nil
       | L_camp, L_imp_ejson =>
         L_camp
@@ -3305,7 +3305,7 @@ Section CompDriver.
           :: L_nnrs
           :: L_nnrs_imp
           :: L_nnrs_imp
-          :: L_imp_qcert
+          :: L_imp_data
           :: L_imp_ejson
           :: nil
       | L_camp, L_js_ast =>
@@ -3317,7 +3317,7 @@ Section CompDriver.
           :: L_nnrs
           :: L_nnrs_imp
           :: L_nnrs_imp
-          :: L_imp_qcert
+          :: L_imp_data
           :: L_imp_ejson
           :: L_js_ast
           :: nil
@@ -3413,7 +3413,7 @@ Section CompDriver.
           :: L_nnrs
           :: L_nnrs_imp
           :: L_nnrs_imp
-          :: L_imp_qcert
+          :: L_imp_data
           :: L_imp_ejson
           :: L_js_ast
           :: L_javascript
@@ -3453,7 +3453,7 @@ Section CompDriver.
           :: L_nnrs_imp
           :: L_nnrs_imp
           :: nil
-      | L_oql, L_imp_qcert =>
+      | L_oql, L_imp_data =>
         L_oql
           :: L_nraenv
           :: L_nraenv
@@ -3462,7 +3462,7 @@ Section CompDriver.
           :: L_nnrs
           :: L_nnrs_imp
           :: L_nnrs_imp
-          :: L_imp_qcert
+          :: L_imp_data
           :: nil
       | L_oql, L_imp_ejson =>
         L_oql
@@ -3473,7 +3473,7 @@ Section CompDriver.
           :: L_nnrs
           :: L_nnrs_imp
           :: L_nnrs_imp
-          :: L_imp_qcert
+          :: L_imp_data
           :: L_imp_ejson
           :: nil
       | L_oql, L_js_ast =>
@@ -3485,7 +3485,7 @@ Section CompDriver.
           :: L_nnrs
           :: L_nnrs_imp
           :: L_nnrs_imp
-          :: L_imp_qcert
+          :: L_imp_data
           :: L_imp_ejson
           :: L_js_ast
           :: nil
@@ -3582,7 +3582,7 @@ Section CompDriver.
           :: L_nnrs
           :: L_nnrs_imp
           :: L_nnrs_imp
-          :: L_imp_qcert
+          :: L_imp_data
           :: L_imp_ejson
           :: L_js_ast
           :: L_javascript
@@ -3622,7 +3622,7 @@ Section CompDriver.
           :: L_nnrs_imp
           :: L_nnrs_imp
           :: nil
-      | L_sql, L_imp_qcert =>
+      | L_sql, L_imp_data =>
         L_sql
           :: L_nraenv
           :: L_nraenv
@@ -3631,7 +3631,7 @@ Section CompDriver.
           :: L_nnrs
           :: L_nnrs_imp
           :: L_nnrs_imp
-          :: L_imp_qcert
+          :: L_imp_data
           :: nil
       | L_sql, L_imp_ejson =>
         L_sql
@@ -3642,7 +3642,7 @@ Section CompDriver.
           :: L_nnrs
           :: L_nnrs_imp
           :: L_nnrs_imp
-          :: L_imp_qcert
+          :: L_imp_data
           :: L_imp_ejson
           :: nil
       | L_sql, L_js_ast =>
@@ -3654,7 +3654,7 @@ Section CompDriver.
           :: L_nnrs
           :: L_nnrs_imp
           :: L_nnrs_imp
-          :: L_imp_qcert
+          :: L_imp_data
           :: L_imp_ejson
           :: L_js_ast
           :: nil
@@ -3751,7 +3751,7 @@ Section CompDriver.
           :: L_nnrs
           :: L_nnrs_imp
           :: L_nnrs_imp
-          :: L_imp_qcert
+          :: L_imp_data
           :: L_imp_ejson
           :: L_js_ast
           :: L_javascript
@@ -3791,7 +3791,7 @@ Section CompDriver.
           :: L_nnrs_imp
           :: L_nnrs_imp
           :: nil
-      | L_sqlpp, L_imp_qcert =>
+      | L_sqlpp, L_imp_data =>
         L_sqlpp
           :: L_nraenv
           :: L_nraenv
@@ -3800,7 +3800,7 @@ Section CompDriver.
           :: L_nnrs
           :: L_nnrs_imp
           :: L_nnrs_imp
-          :: L_imp_qcert
+          :: L_imp_data
           :: nil
       | L_sqlpp, L_imp_ejson =>
         L_sqlpp
@@ -3811,7 +3811,7 @@ Section CompDriver.
           :: L_nnrs
           :: L_nnrs_imp
           :: L_nnrs_imp
-          :: L_imp_qcert
+          :: L_imp_data
           :: L_imp_ejson
           :: nil
       | L_sqlpp, L_js_ast =>
@@ -3823,7 +3823,7 @@ Section CompDriver.
           :: L_nnrs
           :: L_nnrs_imp
           :: L_nnrs_imp
-          :: L_imp_qcert
+          :: L_imp_data
           :: L_imp_ejson
           :: L_js_ast
           :: nil
@@ -3920,7 +3920,7 @@ Section CompDriver.
           :: L_nnrs
           :: L_nnrs_imp
           :: L_nnrs_imp
-          :: L_imp_qcert
+          :: L_imp_data
           :: L_imp_ejson
           :: L_js_ast
           :: L_javascript
@@ -3960,7 +3960,7 @@ Section CompDriver.
           :: L_nnrs_imp
           :: L_nnrs_imp
           :: nil
-      | L_lambda_nra, L_imp_qcert =>
+      | L_lambda_nra, L_imp_data =>
         L_lambda_nra
           :: L_nraenv
           :: L_nraenv
@@ -3969,7 +3969,7 @@ Section CompDriver.
           :: L_nnrs
           :: L_nnrs_imp
           :: L_nnrs_imp
-          :: L_imp_qcert
+          :: L_imp_data
           :: nil
       | L_lambda_nra, L_imp_ejson =>
         L_lambda_nra
@@ -3980,7 +3980,7 @@ Section CompDriver.
           :: L_nnrs
           :: L_nnrs_imp
           :: L_nnrs_imp
-          :: L_imp_qcert
+          :: L_imp_data
           :: L_imp_ejson
           :: nil
       | L_lambda_nra, L_js_ast =>
@@ -3992,7 +3992,7 @@ Section CompDriver.
           :: L_nnrs
           :: L_nnrs_imp
           :: L_nnrs_imp
-          :: L_imp_qcert
+          :: L_imp_data
           :: L_imp_ejson
           :: L_js_ast
           :: nil
@@ -4080,7 +4080,7 @@ Section CompDriver.
           :: L_nnrs
           :: L_nnrs_imp
           :: L_nnrs_imp
-          :: L_imp_qcert
+          :: L_imp_data
           :: L_imp_ejson
           :: L_js_ast
           :: L_javascript
@@ -4124,7 +4124,7 @@ Section CompDriver.
           :: L_nnrs_imp
           :: L_nnrs_imp
           :: nil
-      | L_nra, L_imp_qcert =>
+      | L_nra, L_imp_data =>
         L_nra
           :: L_nraenv_core
           :: L_nraenv
@@ -4134,7 +4134,7 @@ Section CompDriver.
           :: L_nnrs
           :: L_nnrs_imp
           :: L_nnrs_imp
-          :: L_imp_qcert
+          :: L_imp_data
           :: nil
       | L_nra, L_imp_ejson =>
         L_nra
@@ -4146,7 +4146,7 @@ Section CompDriver.
           :: L_nnrs
           :: L_nnrs_imp
           :: L_nnrs_imp
-          :: L_imp_qcert
+          :: L_imp_data
           :: L_imp_ejson
           :: nil
       | L_nra, L_js_ast =>
@@ -4159,7 +4159,7 @@ Section CompDriver.
           :: L_nnrs
           :: L_nnrs_imp
           :: L_nnrs_imp
-          :: L_imp_qcert
+          :: L_imp_data
           :: L_imp_ejson
           :: L_js_ast
           :: nil
@@ -4247,7 +4247,7 @@ Section CompDriver.
           :: L_nnrs
           :: L_nnrs_imp
           :: L_nnrs_imp
-          :: L_imp_qcert
+          :: L_imp_data
           :: L_imp_ejson
           :: L_js_ast
           :: L_javascript
@@ -4287,7 +4287,7 @@ Section CompDriver.
           :: L_nnrs_imp
           :: L_nnrs_imp
           :: nil
-      | L_nraenv_core, L_imp_qcert =>
+      | L_nraenv_core, L_imp_data =>
         L_nraenv_core
           :: L_nraenv
           :: L_nraenv
@@ -4296,7 +4296,7 @@ Section CompDriver.
           :: L_nnrs
           :: L_nnrs_imp
           :: L_nnrs_imp
-          :: L_imp_qcert
+          :: L_imp_data
           :: nil
       | L_nraenv_core, L_imp_ejson =>
         L_nraenv_core
@@ -4307,7 +4307,7 @@ Section CompDriver.
           :: L_nnrs
           :: L_nnrs_imp
           :: L_nnrs_imp
-          :: L_imp_qcert
+          :: L_imp_data
           :: L_imp_ejson
           :: nil
       | L_nraenv_core, L_js_ast =>
@@ -4319,7 +4319,7 @@ Section CompDriver.
           :: L_nnrs
           :: L_nnrs_imp
           :: L_nnrs_imp
-          :: L_imp_qcert
+          :: L_imp_data
           :: L_imp_ejson
           :: L_js_ast
           :: nil
@@ -4406,7 +4406,7 @@ Section CompDriver.
           :: L_nnrs
           :: L_nnrs_imp
           :: L_nnrs_imp
-          :: L_imp_qcert
+          :: L_imp_data
           :: L_imp_ejson
           :: L_js_ast
           :: L_javascript
@@ -4442,7 +4442,7 @@ Section CompDriver.
           :: L_nnrs_imp
           :: L_nnrs_imp
           :: nil
-      | L_nraenv, L_imp_qcert =>
+      | L_nraenv, L_imp_data =>
         L_nraenv
           :: L_nraenv
           :: L_nnrc
@@ -4450,7 +4450,7 @@ Section CompDriver.
           :: L_nnrs
           :: L_nnrs_imp
           :: L_nnrs_imp
-          :: L_imp_qcert
+          :: L_imp_data
           :: nil
       | L_nraenv, L_imp_ejson =>
         L_nraenv
@@ -4460,7 +4460,7 @@ Section CompDriver.
           :: L_nnrs
           :: L_nnrs_imp
           :: L_nnrs_imp
-          :: L_imp_qcert
+          :: L_imp_data
           :: L_imp_ejson
           :: nil
       | L_nraenv, L_js_ast =>
@@ -4471,7 +4471,7 @@ Section CompDriver.
           :: L_nnrs
           :: L_nnrs_imp
           :: L_nnrs_imp
-          :: L_imp_qcert
+          :: L_imp_data
           :: L_imp_ejson
           :: L_js_ast
           :: nil
@@ -4546,7 +4546,7 @@ Section CompDriver.
           :: L_nnrs
           :: L_nnrs_imp
           :: L_nnrs_imp
-          :: L_imp_qcert
+          :: L_imp_data
           :: L_imp_ejson
           :: L_js_ast
           :: L_javascript
@@ -4578,14 +4578,14 @@ Section CompDriver.
           :: L_nnrs_imp
           :: L_nnrs_imp
           :: nil
-      | L_nnrc_core, L_imp_qcert =>
+      | L_nnrc_core, L_imp_data =>
         L_nnrc_core
           :: L_nnrc
           :: L_nnrc
           :: L_nnrs
           :: L_nnrs_imp
           :: L_nnrs_imp
-          :: L_imp_qcert
+          :: L_imp_data
           :: nil
       | L_nnrc_core, L_imp_ejson =>
         L_nnrc_core
@@ -4594,7 +4594,7 @@ Section CompDriver.
           :: L_nnrs
           :: L_nnrs_imp
           :: L_nnrs_imp
-          :: L_imp_qcert
+          :: L_imp_data
           :: L_imp_ejson
           :: nil
       | L_nnrc_core, L_js_ast =>
@@ -4604,7 +4604,7 @@ Section CompDriver.
           :: L_nnrs
           :: L_nnrs_imp
           :: L_nnrs_imp
-          :: L_imp_qcert
+          :: L_imp_data
           :: L_imp_ejson
           :: L_js_ast
           :: nil
@@ -4683,7 +4683,7 @@ Section CompDriver.
           :: L_nnrs
           :: L_nnrs_imp
           :: L_nnrs_imp
-          :: L_imp_qcert
+          :: L_imp_data
           :: L_imp_ejson
           :: L_js_ast
           :: L_javascript
@@ -4711,13 +4711,13 @@ Section CompDriver.
           :: L_nnrs_imp
           :: L_nnrs_imp
           :: nil
-      | L_nnrc, L_imp_qcert =>
+      | L_nnrc, L_imp_data =>
         L_nnrc
           :: L_nnrc
           :: L_nnrs
           :: L_nnrs_imp
           :: L_nnrs_imp
-          :: L_imp_qcert
+          :: L_imp_data
           :: nil
       | L_nnrc, L_imp_ejson =>
         L_nnrc
@@ -4725,7 +4725,7 @@ Section CompDriver.
           :: L_nnrs
           :: L_nnrs_imp
           :: L_nnrs_imp
-          :: L_imp_qcert
+          :: L_imp_data
           :: L_imp_ejson
           :: nil
       | L_nnrc, L_js_ast =>
@@ -4734,7 +4734,7 @@ Section CompDriver.
           :: L_nnrs
           :: L_nnrs_imp
           :: L_nnrs_imp
-          :: L_imp_qcert
+          :: L_imp_data
           :: L_imp_ejson
           :: L_js_ast
           :: nil
@@ -4773,24 +4773,24 @@ Section CompDriver.
           :: L_nnrs_imp
           :: L_nnrs_imp
           :: nil
-      | L_nnrs, L_imp_qcert =>
+      | L_nnrs, L_imp_data =>
         L_nnrs
           :: L_nnrs_imp
           :: L_nnrs_imp
-          :: L_imp_qcert
+          :: L_imp_data
           :: nil
       | L_nnrs, L_imp_ejson =>
         L_nnrs
           :: L_nnrs_imp
           :: L_nnrs_imp
-          :: L_imp_qcert
+          :: L_imp_data
           :: L_imp_ejson
           :: nil
       | L_nnrs, L_js_ast =>
         L_nnrs
           :: L_nnrs_imp
           :: L_nnrs_imp
-          :: L_imp_qcert
+          :: L_imp_data
           :: L_imp_ejson
           :: L_js_ast
           :: nil
@@ -4798,7 +4798,7 @@ Section CompDriver.
         L_nnrs
           :: L_nnrs_imp
           :: L_nnrs_imp
-          :: L_imp_qcert
+          :: L_imp_data
           :: L_imp_ejson
           :: L_js_ast
           :: L_javascript
@@ -4817,19 +4817,19 @@ Section CompDriver.
           :: L_nnrs_imp
           :: L_nnrs_imp
           :: nil
-      | L_nnrs_core, L_imp_qcert =>
+      | L_nnrs_core, L_imp_data =>
         L_nnrs_core
           :: L_nnrs
           :: L_nnrs_imp
           :: L_nnrs_imp
-          :: L_imp_qcert
+          :: L_imp_data
           :: nil
       | L_nnrs_core, L_imp_ejson =>
         L_nnrs_core
           :: L_nnrs
           :: L_nnrs_imp
           :: L_nnrs_imp
-          :: L_imp_qcert
+          :: L_imp_data
           :: L_imp_ejson
           :: nil
       | L_nnrs_core, L_js_ast =>
@@ -4837,7 +4837,7 @@ Section CompDriver.
           :: L_nnrs
           :: L_nnrs_imp
           :: L_nnrs_imp
-          :: L_imp_qcert
+          :: L_imp_data
           :: L_imp_ejson
           :: L_js_ast
           :: nil
@@ -4846,7 +4846,7 @@ Section CompDriver.
           :: L_nnrs
           :: L_nnrs_imp
           :: L_nnrs_imp
-          :: L_imp_qcert
+          :: L_imp_data
           :: L_imp_ejson
           :: L_js_ast
           :: L_javascript
@@ -4856,47 +4856,47 @@ Section CompDriver.
         L_nnrs_imp
           :: L_nnrs_imp
           :: nil
-      | L_nnrs_imp, L_imp_qcert =>
+      | L_nnrs_imp, L_imp_data =>
         L_nnrs_imp
           :: L_nnrs_imp
-          :: L_imp_qcert
+          :: L_imp_data
           :: nil
       | L_nnrs_imp, L_imp_ejson =>
         L_nnrs_imp
           :: L_nnrs_imp
-          :: L_imp_qcert
+          :: L_imp_data
           :: L_imp_ejson
           :: nil
       | L_nnrs_imp, L_js_ast =>
         L_nnrs_imp
           :: L_nnrs_imp
-          :: L_imp_qcert
+          :: L_imp_data
           :: L_imp_ejson
           :: L_js_ast
           :: nil
       | L_nnrs_imp, L_javascript =>
         L_nnrs_imp
           :: L_nnrs_imp
-          :: L_imp_qcert
+          :: L_imp_data
           :: L_imp_ejson
           :: L_js_ast
           :: L_javascript
           :: nil
-      (* From imp_qcert: *)
-      | L_imp_qcert, L_imp_qcert =>
-        L_imp_qcert
+      (* From imp_data: *)
+      | L_imp_data, L_imp_data =>
+        L_imp_data
           :: nil
-      | L_imp_qcert, L_imp_ejson =>
-        L_imp_qcert
+      | L_imp_data, L_imp_ejson =>
+        L_imp_data
           :: L_imp_ejson
           :: nil
-      | L_imp_qcert, L_js_ast =>
-        L_imp_qcert
+      | L_imp_data, L_js_ast =>
+        L_imp_data
           :: L_imp_ejson
           :: L_js_ast
           :: nil
-      | L_imp_qcert, L_javascript =>
-        L_imp_qcert
+      | L_imp_data, L_javascript =>
+        L_imp_data
           :: L_imp_ejson
           :: L_js_ast
           :: L_javascript
@@ -4975,7 +4975,7 @@ Section CompDriver.
           :: L_nnrs_imp
           :: L_nnrs_imp
           :: nil
-      | L_nnrcmr, L_imp_qcert =>
+      | L_nnrcmr, L_imp_data =>
         L_nnrcmr
           :: L_nnrcmr
           :: L_nnrc
@@ -4983,7 +4983,7 @@ Section CompDriver.
           :: L_nnrs
           :: L_nnrs_imp
           :: L_nnrs_imp
-          :: L_imp_qcert
+          :: L_imp_data
           :: nil
       | L_nnrcmr, L_imp_ejson =>
         L_nnrcmr
@@ -4993,7 +4993,7 @@ Section CompDriver.
           :: L_nnrs
           :: L_nnrs_imp
           :: L_nnrs_imp
-          :: L_imp_qcert
+          :: L_imp_data
           :: L_imp_ejson
           :: nil
       | L_nnrcmr, L_js_ast =>
@@ -5004,7 +5004,7 @@ Section CompDriver.
           :: L_nnrs
           :: L_nnrs_imp
           :: L_nnrs_imp
-          :: L_imp_qcert
+          :: L_imp_data
           :: L_imp_ejson
           :: L_js_ast
           :: nil
@@ -5016,7 +5016,7 @@ Section CompDriver.
           :: L_nnrs
           :: L_nnrs_imp
           :: L_nnrs_imp
-          :: L_imp_qcert
+          :: L_imp_data
           :: L_imp_ejson
           :: L_js_ast
           :: L_javascript
@@ -5216,14 +5216,14 @@ Section CompDriver.
 
     Hint Resolve exists_path_from_source_target_completeness_imp_ejson : exists_path_hints.
 
-    Lemma exists_path_from_source_target_completeness_imp_qcert :
+    Lemma exists_path_from_source_target_completeness_imp_data :
       (forall dv,
-          exists_path_from_source_target L_imp_qcert (target_language_of_driver (Dv_imp_qcert dv))).
+          exists_path_from_source_target L_imp_data (target_language_of_driver (Dv_imp_data dv))).
     Proof.
       induction dv; prove_exists_path_complete.
     Qed.
 
-    Hint Resolve exists_path_from_source_target_completeness_imp_qcert : exists_path_hints.
+    Hint Resolve exists_path_from_source_target_completeness_imp_data : exists_path_hints.
 
     Lemma exists_path_from_source_target_completeness_nnrs_imp :
       (forall dv,
