compiler/core/Driver/CompEval.v
@@ -125,9 +125,9 @@ Section CompEval.
     Definition eval_nnrs_imp (q:nnrs_imp) (cenv: bindings) : option data :=
       NNRSimpEval.nnrs_imp_eval_top h cenv q.
 
-    (* Language: imp_qcert *)
-    Definition eval_imp_qcert (q:imp_qcert) (cenv: bindings) : option data :=
-      ImpQcertEval.imp_qcert_eval_top h cenv q.
+    (* Language: imp_data *)
+    Definition eval_imp_data (q:imp_data) (cenv: bindings) : option data :=
+      ImpDataEval.imp_data_eval_top h cenv q.
 
     (* Language: imp_ejson *)
     (* XXX Is this really what we want to wrap/unwrap in data? *)
@@ -185,7 +185,7 @@ Section CompEval.
       | Q_nnrs_core q => lift_output (eval_nnrs_core q (lift_input ev_in))
       | Q_nnrs q => lift_output (eval_nnrs q (lift_input ev_in))
       | Q_nnrs_imp q => lift_output (eval_nnrs_imp q (lift_input ev_in))
-      | Q_imp_qcert q => lift_output (eval_imp_qcert q (lift_input ev_in))
+      | Q_imp_data q => lift_output (eval_imp_data q (lift_input ev_in))
       | Q_imp_ejson q => lift_output (eval_imp_ejson q (lift_input ev_in))
       | Q_nnrcmr q => lift_output (eval_nnrcmr q ev_in) (* XXX Does not localize, keeps distributed information XXX *)
       | Q_dnnrc q => lift_output (eval_dnnrc q ev_in) (* XXX Does not localize, keeps distributed information XXX *)
@@ -215,7 +215,7 @@ Section CompEval.
       | Q_nnrs_core _ => Ev_out_unsupported ("No debug evaluation support for "++(name_of_language (language_of_query q)))
       | Q_nnrs _ => Ev_out_unsupported ("No debug evaluation support for "++(name_of_language (language_of_query q)))
       | Q_nnrs_imp _ => Ev_out_unsupported ("No debug evaluation support for "++(name_of_language (language_of_query q)))
-      | Q_imp_qcert _ => Ev_out_unsupported ("No debug evaluation support for "++(name_of_language (language_of_query q)))
+      | Q_imp_data _ => Ev_out_unsupported ("No debug evaluation support for "++(name_of_language (language_of_query q)))
       | Q_imp_ejson _ => Ev_out_unsupported ("No debug evaluation support for "++(name_of_language (language_of_query q)))
       | Q_nnrcmr _ => Ev_out_unsupported ("No debug evaluation support for "++(name_of_language (language_of_query q)))
       | Q_dnnrc _ => Ev_out_unsupported ("No debug evaluation support for "++(name_of_language (language_of_query q)))
